AlgoLib/Experimental/RAM/Prototype/Composition.lean
@@ -3,7 +3,8 @@ Copyright (c) 2026 Sorrachai Yingchareonthawornchai. All rights reserved.
 Released under Apache 2.0 license as described in the file LICENSE.
 Authors: Sorrachai Yingchareonthawornchai
 -/
-import AlgoLib.Experimental.RAM.Prototype.Composition.Language
+import AlgoLib.Experimental.RAM.Prototype.LogicalFrontend
+import AlgoLib.Experimental.RAM.Prototype.Composition.Contracts
 import AlgoLib.Experimental.RAM.Prototype.Composition.Loom
 import AlgoLib.Experimental.RAM.Prototype.Composition.Compatibility
 
